path.v
@@ -3,53 +3,63 @@
 Require Import Utf8 PeanoNat Wf_nat List Lia.
 From larith Require Import tactics notations utilities.
 
-Section Path_predicate.
+Section Graph_connectivity.
 
 Variable node : Type.
 Variable adj : node -> list node.
-Variable Terminal : node -> Prop.
+Variable End : node -> Prop.
 
 Hypothesis dec : ∀v w : node, {v = w} + {v ≠ w}.
-Hypothesis Terminal_dec : ∀v, {Terminal v} + {¬Terminal v}.
+Hypothesis End_dec : ∀v, {End v} + {¬End v}.
 
-(* There exists a path to a terminal node in graph g. *)
-Inductive Path g : node -> Prop :=
-  | Path_finish v : Terminal v -> Path g v
-  | Path_step v w : In w g -> In w (adj v) -> Path g w -> Path g v.
+(* A path to an end node in graph g. *)
+Inductive path g : node -> Type :=
+  | path_stop v : End v -> path g v
+  | path_step v w : In w g -> In w (adj v) -> path g w -> path g v.
 
-Lemma Path_subset g g' v :
-  Path g' v -> (∀x, In x g' -> In x g) -> Path g v.
+Inductive Connected g v : Prop :=
+  | conn : path g v -> Connected g v.
+
+Fixpoint path_length {g n} (p : path g n) : nat :=
+  match p with
+  | path_stop _ _ _ => 0
+  | path_step _ _ _ _ _ q => S (path_length q)
+  end.
+
+Lemma path_subset g g' v :
+  path g' v -> (∀x, In x g' -> In x g) -> path g v.
 Proof.
-intros path subset; induction path.
-now apply Path_finish. eapply Path_step.
-apply subset, H. all: easy.
+intros p subset; induction p.
+now apply path_stop. eapply path_step.
+apply subset, i. all: easy.
 Qed.
 
-Lemma Path_split g g1 g2 v :
-  Path g v -> (∀x, In x g <-> In x g1 \/ In x g2) ->
-  Exists (Path g1) g2 \/ Path g1 v.
+Lemma Connected_split g g1 g2 v :
+  Connected g v -> (∀x, In x g <-> In x g1 \/ In x g2) ->
+  Exists (Connected g1) g2 \/ Connected g1 v.
 Proof.
-intros path g_spec; induction path.
-- right; now apply Path_finish.
-- destruct IHpath. now left.
-  apply g_spec in H as [H|H].
-  + right; now apply Path_step with (w:=w).
-  + left; apply Exists_exists; now exists w.
+intros [p] g_spec; induction p.
+- right; apply conn, path_stop, e.
+- destruct IHp. now left. destruct H.
+  apply g_spec in i as [H1|H2].
+  + right; now apply conn, path_step with (w:=w).
+  + left; apply Exists_exists; exists w; split.
+    easy. apply conn, X.
 Qed.
 
-Theorem Path_dec g v :
-  {Path g v} + {¬Path g v}.
+Theorem Connected_dec g v :
+  {Connected g v} + {¬Connected g v}.
 Proof.
 remember (length g) as n; revert Heqn; revert g v.
 apply lt_wf_rect with (n:=n); clear n; intros n IH g v g_len.
 (* Check if v is a target state. *)
-destruct (Terminal_dec v).
-left; now apply Path_finish.
+destruct (End_dec v).
+left; apply conn, path_stop, e.
 (* Determine if there is an intersection between g and adj v. *)
 pose(gv := intersect dec g (adj v)).
 destruct (Nat.eq_dec (length gv) 0).
 - (* No path exists since g ∩ adj v = ∅. *)
-  right; intros HC; inv HC. apply in_nil with (a:=w).
+  right; intros [p]; inv p. apply in_nil with (a:=w).
   apply length_zero_iff_nil in e; rewrite <-e.
   now apply intersect_spec.
 - (* Show that g is not empty. *)
@@ -57,22 +67,22 @@ destruct (Nat.eq_dec (length gv) 0).
     intros H; apply n1. unfold gv; rewrite intersect_length. lia. }
   (* Determine if a node in g ∩ adj v is connected through g \ adj v. *)
   pose(g' := subtract dec g (adj v)).
-  destruct (Exists_dec (Path g') gv).
+  destruct (Exists_dec (Connected g') gv).
   + (* Decide using the induction hypothesis. *)
     intros; eapply IH. 2: reflexivity.
     unfold g'; rewrite g_len, subtract_length.
     fold gv; lia.
   + (* A path exists. *)
-    left. apply Exists_exists in e as [w [H1w H2w]].
+    left. apply Exists_exists in e as [w [H1w [p]]].
     apply intersect_spec in H1w.
-    apply Path_step with (w:=w); try easy.
-    eapply Path_subset. apply H2w.
+    apply conn, path_step with (w:=w); try easy.
+    eapply path_subset. apply p.
     intros; eapply subtract_spec, H0.
   + (* Any path would yield a contradiction. *)
     right. intros Hv; apply n2.
-    apply Path_split with (g1:=g')(g2:=gv) in Hv as [Hv|Hv].
+    apply Connected_split with (g1:=g')(g2:=gv) in Hv as [Hv|[p]].
     (* Either we find a path through g', or we find an impossible path. *)
-    easy. exfalso; inv Hv. apply subtract_spec in H0; easy.
+    easy. exfalso; inv p. apply subtract_spec in H0; easy.
     (* Show that g = g1 ∪ g2. *)
     intros w; split; intros.
     * destruct (in_dec dec w (adj v)).
@@ -83,6 +93,7 @@ destruct (Nat.eq_dec (length gv) 0).
       now apply intersect_spec in H0.
 Qed.
 
-End Path_predicate.
+End Graph_connectivity.
 
-Arguments Path {_}.
+Arguments path {_}.
+Arguments Connected {_}.
